Hoare simulation bind rule

proofmode/HSim.v
@@ -232,141 +232,6 @@ Section SIM.
       _hsim hsim Q ctx fuel true true (st_src, itr_src) (st_tgt, itr_tgt)
   .
 
-  Inductive _hsim
-            (hsim: forall R_src R_tgt
-                          (Q: Any.t -> Any.t -> R_src -> R_tgt -> iProp)
-                          (ctx: Σ),
-                option Ord.t -> bool -> bool -> Any.t * itree hEs R_src -> Any.t * itree Es R_tgt -> Prop)
-            {R_src R_tgt}
-            (Q: Any.t -> Any.t -> R_src -> R_tgt -> iProp)
-            (ctx: Σ)
-    : option Ord.t -> bool -> bool -> Any.t * itree hEs R_src -> Any.t * itree Es R_tgt -> Prop :=
-  | hsim_ret
-      v_src v_tgt
-      st_src st_tgt
-      fuel f_src f_tgt
-      (RET: current_iProp ctx (Q st_src st_tgt v_src v_tgt))
-    :
-      _hsim hsim Q ctx fuel f_src f_tgt (st_src, (Ret v_src)) (st_tgt, (Ret v_tgt))
-  | hsim_call
-      fsp (x: fsp.(meta)) w0 FR
-      fn arg_src arg_tgt
-      st_src0 st_tgt0 ktr_src ktr_tgt
-      fuel f_src f_tgt
-      (SPEC: stb fn = Some fsp)
-      (PRE: current_iProp ctx (FR ** I w0 st_src0 st_tgt0 ** fsp.(precond) (Some mn) x arg_src arg_tgt))
-      (MEASURE: o = ord_top)
-      (NPURE: fsp.(measure) x = ord_top)
-      (POST: forall ctx1 w1 st_src1 st_tgt1 ret_src ret_tgt
-                    (ACC: current_iProp ctx1 (FR ** I w1 st_src1 st_tgt1 ** fsp.(postcond) (Some mn) x ret_src ret_tgt)),
-          hsim _ _ Q ctx1 None true true (st_src1, ktr_src ret_src) (st_tgt1, ktr_tgt ret_tgt))
-    :
-      _hsim hsim Q ctx fuel f_src f_tgt (st_src0, trigger (Call fn arg_src) >>= ktr_src) (st_tgt0, trigger (Call fn arg_tgt) >>= ktr_tgt)
-  | hsim_apc_start
-      fuel1
-      st_src st_tgt ktr_src itr_tgt
-      fuel f_src f_tgt
-      (SIM: _hsim hsim Q ctx (fuel1) true f_tgt (st_src, ktr_src tt) (st_tgt, itr_tgt))
-    :
-      _hsim hsim Q ctx fuel f_src f_tgt (st_src, trigger (hAPC) >>= ktr_src) (st_tgt, itr_tgt)
-  | hsim_apc_step
-      fsp (x: fsp.(meta)) w0 FR arg_src
-      fn arg_tgt
-      st_src0 st_tgt0 itr_src ktr_tgt
-      fuel0 f_src f_tgt
-      (SPEC: stb fn = Some fsp)
-      (PRE: current_iProp ctx (FR ** I w0 st_src0 st_tgt0 ** fsp.(precond) (Some mn) x arg_src arg_tgt))
-      (MEASURE: ord_lt (fsp.(measure) x) o)
-      (PURE: is_pure (fsp.(measure) x))
-      (POST: exists fuel1,
-          (<<FUEL: Ord.lt fuel1 fuel0>>) /\
-          (<<SIM: forall ctx1 w1 st_src1 st_tgt1 ret_src ret_tgt
-                         (ACC: current_iProp ctx1 (FR ** I w1 st_src1 st_tgt1 ** fsp.(postcond) (Some mn) x ret_src ret_tgt)),
-              hsim _ _ Q ctx1 (Some fuel1) true true (st_src1, itr_src) (st_tgt1, ktr_tgt ret_tgt)>>))
-    :
-      _hsim hsim Q ctx (Some fuel0) f_src f_tgt (st_src0, itr_src) (st_tgt0, trigger (Call fn arg_tgt) >>= ktr_tgt)
-  | hsim_syscall
-      fn arg rvs
-      st_src st_tgt ktr_src ktr_tgt
-      fuel f_src f_tgt
-      (POST: forall ret,
-          hsim _ _ Q ctx None true true (st_src, ktr_src ret) (st_tgt, ktr_tgt ret))
-    :
-      _hsim hsim Q ctx fuel f_src f_tgt (st_src, trigger (Syscall fn arg rvs) >>= ktr_src) (st_tgt, trigger (Syscall fn arg rvs) >>= ktr_tgt)
-  | hsim_tau_src
-      st_src st_tgt itr_src itr_tgt
-      fuel f_src f_tgt
-      (SIM: _hsim hsim Q ctx None true f_tgt (st_src, itr_src) (st_tgt, itr_tgt))
-    :
-      _hsim hsim Q ctx fuel f_src f_tgt (st_src, tau;; itr_src) (st_tgt, itr_tgt)
-  | hsim_tau_tgt
-      st_src st_tgt itr_src itr_tgt
-      fuel f_src f_tgt
-      (SIM: _hsim hsim Q ctx fuel f_src true (st_src, itr_src) (st_tgt, itr_tgt))
-    :
-      _hsim hsim Q ctx fuel f_src f_tgt (st_src, itr_src) (st_tgt, tau;; itr_tgt)
-  | hsim_choose_src
-      X
-      st_src st_tgt ktr_src itr_tgt
-      fuel f_src f_tgt
-      (SIM: exists x, _hsim hsim Q ctx None true f_tgt (st_src, ktr_src x) (st_tgt, itr_tgt))
-    :
-      _hsim hsim Q ctx fuel f_src f_tgt (st_src, trigger (Choose X) >>= ktr_src) (st_tgt, itr_tgt)
-  | hsim_choose_tgt
-      X
-      st_src st_tgt itr_src ktr_tgt
-      fuel f_src f_tgt
-      (SIM: forall x, _hsim hsim Q ctx fuel f_src true (st_src, itr_src) (st_tgt, ktr_tgt x))
-    :
-      _hsim hsim Q ctx fuel f_src f_tgt (st_src, itr_src) (st_tgt, trigger (Choose X) >>= ktr_tgt)
-  | hsim_take_src
-      X
-      st_src st_tgt ktr_src itr_tgt
-      fuel f_src f_tgt
-      (SIM: forall x, _hsim hsim Q ctx None true f_tgt (st_src, ktr_src x) (st_tgt, itr_tgt))
-    :
-      _hsim hsim Q ctx fuel f_src f_tgt (st_src, trigger (Take X) >>= ktr_src) (st_tgt, itr_tgt)
-  | hsim_take_tgt
-      X
-      st_src st_tgt itr_src ktr_tgt
-      fuel f_src f_tgt
-      (SIM: exists x, _hsim hsim Q ctx fuel f_src true (st_src, itr_src) (st_tgt, ktr_tgt x))
-    :
-      _hsim hsim Q ctx fuel f_src f_tgt (st_src, itr_src) (st_tgt, trigger (Take X) >>= ktr_tgt)
-  | hsim_pput_src
-      st_src1
-      st_src0 st_tgt ktr_src itr_tgt
-      fuel f_src f_tgt
-      (SIM: _hsim hsim Q ctx None true f_tgt (st_src1, ktr_src tt) (st_tgt, itr_tgt))
-    :
-      _hsim hsim Q ctx fuel f_src f_tgt (st_src0, trigger (PPut st_src1) >>= ktr_src) (st_tgt, itr_tgt)
-  | hsim_pput_tgt
-      st_tgt1
-      st_src st_tgt0 itr_src ktr_tgt
-      fuel f_src f_tgt
-      (SIM: _hsim hsim Q ctx fuel f_src true (st_src, itr_src) (st_tgt1, ktr_tgt tt))
-    :
-      _hsim hsim Q ctx fuel f_src f_tgt (st_src, itr_src) (st_tgt0, trigger (PPut st_tgt1) >>= ktr_tgt)
-  | hsim_pget_src
-      st_src st_tgt ktr_src itr_tgt
-      fuel f_src f_tgt
-      (SIM: _hsim hsim Q ctx None true f_tgt (st_src, ktr_src st_src) (st_tgt, itr_tgt))
-    :
-      _hsim hsim Q ctx fuel f_src f_tgt (st_src, trigger (PGet) >>= ktr_src) (st_tgt, itr_tgt)
-  | hsim_pget_tgt
-      st_src st_tgt itr_src ktr_tgt
-      fuel f_src f_tgt
-      (SIM: _hsim hsim Q ctx fuel f_src true (st_src, itr_src) (st_tgt, ktr_tgt st_tgt))
-    :
-      _hsim hsim Q ctx fuel f_src f_tgt (st_src, itr_src) (st_tgt, trigger (PGet) >>= ktr_tgt)
-  | hsim_progress
-      st_src st_tgt itr_src itr_tgt
-      fuel
-      (SIM: hsim _ _ Q ctx fuel false false (st_src, itr_src) (st_tgt, itr_tgt))
-    :
-      _hsim hsim Q ctx fuel true true (st_src, itr_src) (st_tgt, itr_tgt)
-  .
-
   Lemma _hsim_ind2
         (hsim: forall R_src R_tgt
                       (Q: Any.t -> Any.t -> R_src -> R_tgt -> iProp)
@@ -1013,6 +878,225 @@ Section SIM.
     eapply _hsim_mon; eauto. i. gbase. eapply rclo9_base. auto.
   Qed.
 
+  Variant hsimC
+          (r g: forall R_src R_tgt
+                       (Q: Any.t -> Any.t -> R_src -> R_tgt -> iProp)
+                       (ctx: Σ),
+              option Ord.t -> bool -> bool -> Any.t * itree hEs R_src -> Any.t * itree Es R_tgt -> Prop)
+          {R_src R_tgt}
+          (Q: Any.t -> Any.t -> R_src -> R_tgt -> iProp)
+          (ctx: Σ)
+    : option Ord.t -> bool -> bool -> Any.t * itree hEs R_src -> Any.t * itree Es R_tgt -> Prop :=
+    | hsimC_ret
+        v_src v_tgt
+        st_src st_tgt
+        fuel f_src f_tgt
+        (RET: current_iProp ctx (Q st_src st_tgt v_src v_tgt))
+      :
+      hsimC r g Q ctx fuel f_src f_tgt (st_src, (Ret v_src)) (st_tgt, (Ret v_tgt))
+    | hsimC_call
+        fsp (x: fsp.(meta)) w0 FR
+        fn arg_src arg_tgt
+        st_src0 st_tgt0 ktr_src ktr_tgt
+        fuel f_src f_tgt
+        (SPEC: stb fn = Some fsp)
+        (PRE: current_iProp ctx (FR ** I w0 st_src0 st_tgt0 ** fsp.(precond) (Some mn) x arg_src arg_tgt))
+        (MEASURE: o = ord_top)
+        (NPURE: fsp.(measure) x = ord_top)
+        (POST: forall ctx1 w1 st_src1 st_tgt1 ret_src ret_tgt
+                      (ACC: current_iProp ctx1 (FR ** I w1 st_src1 st_tgt1 ** fsp.(postcond) (Some mn) x ret_src ret_tgt)),
+            g _ _ Q ctx1 None true true (st_src1, ktr_src ret_src) (st_tgt1, ktr_tgt ret_tgt))
+      :
+      hsimC r g Q ctx fuel f_src f_tgt (st_src0, trigger (Call fn arg_src) >>= ktr_src) (st_tgt0, trigger (Call fn arg_tgt) >>= ktr_tgt)
+    | hsimC_apc_start
+        fuel1
+        st_src st_tgt ktr_src itr_tgt
+        fuel f_src f_tgt
+        (SIM: r _ _ Q ctx (fuel1) true f_tgt (st_src, ktr_src tt) (st_tgt, itr_tgt))
+      :
+      hsimC r g Q ctx fuel f_src f_tgt (st_src, trigger (hAPC) >>= ktr_src) (st_tgt, itr_tgt)
+    | hsimC_apc_step
+        fsp (x: fsp.(meta)) w0 FR arg_src
+        fn arg_tgt
+        st_src0 st_tgt0 itr_src ktr_tgt
+        fuel0 f_src f_tgt
+        (SPEC: stb fn = Some fsp)
+        (PRE: current_iProp ctx (FR ** I w0 st_src0 st_tgt0 ** fsp.(precond) (Some mn) x arg_src arg_tgt))
+        (MEASURE: ord_lt (fsp.(measure) x) o)
+        (PURE: is_pure (fsp.(measure) x))
+        (POST: exists fuel1,
+            (<<FUEL: Ord.lt fuel1 fuel0>>) /\
+              (<<SIM: forall ctx1 w1 st_src1 st_tgt1 ret_src ret_tgt
+                             (ACC: current_iProp ctx1 (FR ** I w1 st_src1 st_tgt1 ** fsp.(postcond) (Some mn) x ret_src ret_tgt)),
+                  g _ _ Q ctx1 (Some fuel1) true true (st_src1, itr_src) (st_tgt1, ktr_tgt ret_tgt)>>))
+      :
+      hsimC r g Q ctx (Some fuel0) f_src f_tgt (st_src0, itr_src) (st_tgt0, trigger (Call fn arg_tgt) >>= ktr_tgt)
+    | hsimC_syscall
+        fn arg rvs
+        st_src st_tgt ktr_src ktr_tgt
+        fuel f_src f_tgt
+        (POST: forall ret,
+            g _ _ Q ctx None true true (st_src, ktr_src ret) (st_tgt, ktr_tgt ret))
+      :
+      hsimC r g Q ctx fuel f_src f_tgt (st_src, trigger (Syscall fn arg rvs) >>= ktr_src) (st_tgt, trigger (Syscall fn arg rvs) >>= ktr_tgt)
+    | hsimC_tau_src
+        st_src st_tgt itr_src itr_tgt
+        fuel f_src f_tgt
+        (SIM: r _ _ Q ctx None true f_tgt (st_src, itr_src) (st_tgt, itr_tgt))
+      :
+      hsimC r g Q ctx fuel f_src f_tgt (st_src, tau;; itr_src) (st_tgt, itr_tgt)
+    | hsimC_tau_tgt
+        st_src st_tgt itr_src itr_tgt
+        fuel f_src f_tgt
+        (SIM: r _ _ Q ctx fuel f_src true (st_src, itr_src) (st_tgt, itr_tgt))
+      :
+      hsimC r g Q ctx fuel f_src f_tgt (st_src, itr_src) (st_tgt, tau;; itr_tgt)
+    | hsimC_choose_src
+        X
+        st_src st_tgt ktr_src itr_tgt
+        fuel f_src f_tgt
+        (SIM: exists x, r _ _ Q ctx None true f_tgt (st_src, ktr_src x) (st_tgt, itr_tgt))
+      :
+      hsimC r g Q ctx fuel f_src f_tgt (st_src, trigger (Choose X) >>= ktr_src) (st_tgt, itr_tgt)
+    | hsimC_choose_tgt
+        X
+        st_src st_tgt itr_src ktr_tgt
+        fuel f_src f_tgt
+        (SIM: forall x, r _ _ Q ctx fuel f_src true (st_src, itr_src) (st_tgt, ktr_tgt x))
+      :
+      hsimC r g Q ctx fuel f_src f_tgt (st_src, itr_src) (st_tgt, trigger (Choose X) >>= ktr_tgt)
+    | hsimC_take_src
+        X
+        st_src st_tgt ktr_src itr_tgt
+        fuel f_src f_tgt
+        (SIM: forall x, r _ _ Q ctx None true f_tgt (st_src, ktr_src x) (st_tgt, itr_tgt))
+      :
+      hsimC r g Q ctx fuel f_src f_tgt (st_src, trigger (Take X) >>= ktr_src) (st_tgt, itr_tgt)
+    | hsimC_take_tgt
+        X
+        st_src st_tgt itr_src ktr_tgt
+        fuel f_src f_tgt
+        (SIM: exists x, r _ _ Q ctx fuel f_src true (st_src, itr_src) (st_tgt, ktr_tgt x))
+      :
+      hsimC r g Q ctx fuel f_src f_tgt (st_src, itr_src) (st_tgt, trigger (Take X) >>= ktr_tgt)
+    | hsimC_pput_src
+        st_src1
+        st_src0 st_tgt ktr_src itr_tgt
+        fuel f_src f_tgt
+        (SIM: r _ _ Q ctx None true f_tgt (st_src1, ktr_src tt) (st_tgt, itr_tgt))
+      :
+      hsimC r g Q ctx fuel f_src f_tgt (st_src0, trigger (PPut st_src1) >>= ktr_src) (st_tgt, itr_tgt)
+    | hsimC_pput_tgt
+        st_tgt1
+        st_src st_tgt0 itr_src ktr_tgt
+        fuel f_src f_tgt
+        (SIM: r _ _ Q ctx fuel f_src true (st_src, itr_src) (st_tgt1, ktr_tgt tt))
+      :
+      hsimC r g Q ctx fuel f_src f_tgt (st_src, itr_src) (st_tgt0, trigger (PPut st_tgt1) >>= ktr_tgt)
+    | hsimC_pget_src
+        st_src st_tgt ktr_src itr_tgt
+        fuel f_src f_tgt
+        (SIM: r _ _ Q ctx None true f_tgt (st_src, ktr_src st_src) (st_tgt, itr_tgt))
+      :
+      hsimC r g Q ctx fuel f_src f_tgt (st_src, trigger (PGet) >>= ktr_src) (st_tgt, itr_tgt)
+    | hsimC_pget_tgt
+        st_src st_tgt itr_src ktr_tgt
+        fuel f_src f_tgt
+        (SIM: r _ _ Q ctx fuel f_src true (st_src, itr_src) (st_tgt, ktr_tgt st_tgt))
+      :
+      hsimC r g Q ctx fuel f_src f_tgt (st_src, itr_src) (st_tgt, trigger (PGet) >>= ktr_tgt)
+    | hsimC_progress
+        st_src st_tgt itr_src itr_tgt
+        fuel
+        (SIM: g _ _ Q ctx fuel false false (st_src, itr_src) (st_tgt, itr_tgt))
+      :
+      hsimC r g Q ctx fuel true true (st_src, itr_src) (st_tgt, itr_tgt)
+  .
+
+  Lemma hsim_indC_mon_gen r0 r1 g0 g1
+        (LE0: r0 <9= r1)
+        (LE1: g0 <9= g1)
+    :
+    @hsimC r0 g0 <9= @hsimC r1 g1.
+  Proof.
+    ii. inv PR.
+    { econs 1; eauto. }
+    { econs 2; eauto. }
+    { econs 3; eauto. }
+    { econs 4; eauto. des. esplits; eauto. }
+    { econs 5; eauto. }
+    { econs 6; eauto. }
+    { econs 7; eauto. }
+    { econs 8; eauto. des. esplits; eauto. }
+    { econs 9; eauto. }
+    { econs 10; eauto. }
+    { econs 11; eauto. des. esplits; eauto. }
+    { econs 12; eauto. }
+    { econs 13; eauto. }
+    { econs 14; eauto. }
+    { econs 15; eauto. }
+    { econs 16; eauto. }
+  Qed.
+
+  Lemma hsim_indC_mon: monotone9 (fun r => @hsimC r r).
+  Proof.
+    ii. eapply hsim_indC_mon_gen; eauto.
+  Qed.
+
+  Lemma hsim_indC_spec:
+    (fun r => @hsimC r r) <10= gupaco9 (_hsim) (cpn9 _hsim).
+  Proof.
+    eapply wrespect9_uclo; eauto with paco. econs.
+    { eapply hsim_indC_mon. }
+    i. inv PR.
+    { econs 1; eauto. }
+    { econs 2; eauto. i. eapply rclo9_base. eauto. }
+    { econs 3; eauto. eapply GF in SIM. eapply _hsim_mon; eauto. i. eapply rclo9_base. eauto. }
+    { econs 4; eauto. des. esplits; eauto. i. eapply rclo9_base. eauto. }
+    { econs 5; eauto. i. eapply rclo9_base. eauto. }
+    { econs 6; eauto. eapply _hsim_mon; eauto. i. eapply rclo9_base. eauto. }
+    { econs 7; eauto. eapply _hsim_mon; eauto. i. eapply rclo9_base. eauto. }
+    { econs 8; eauto. des. esplits; eauto. eapply _hsim_mon; eauto. i. eapply rclo9_base. eauto. }
+    { econs 9; eauto. i. eapply _hsim_mon; eauto. i. eapply rclo9_base. eauto. }
+    { econs 10; eauto. i. eapply _hsim_mon; eauto. i. eapply rclo9_base. eauto. }
+    { econs 11; eauto. des. esplits; eauto. eapply _hsim_mon; eauto. i. eapply rclo9_base. eauto. }
+    { econs 12; eauto. eapply _hsim_mon; eauto. i. eapply rclo9_base. eauto. }
+    { econs 13; eauto. eapply _hsim_mon; eauto. i. eapply rclo9_base. eauto. }
+    { econs 14; eauto. eapply _hsim_mon; eauto. i. eapply rclo9_base. eauto. }
+    { econs 15; eauto. eapply _hsim_mon; eauto. i. eapply rclo9_base. eauto. }
+    { econs 16; eauto. eapply rclo9_base. eauto. }
+  Qed.
+
+  Lemma hsimC_spec:
+    hsimC <11= gpaco9 (_hsim) (cpn9 _hsim).
+  Proof.
+    i. inv PR.
+    { gstep. econs 1; eauto. }
+    { gstep. econs 2; eauto. i. gbase. eauto. }
+    { guclo hsim_indC_spec. ss. econs 3; eauto. gbase. eauto. }
+    { gstep. econs 4; eauto. des. esplits; eauto. i. gbase. eauto. }
+    { gstep. econs 5; eauto. i. gbase. eauto. }
+    { guclo hsim_indC_spec. ss. econs 6; eauto. gbase. eauto. }
+    { guclo hsim_indC_spec. ss. econs 7; eauto. gbase. eauto. }
+    { guclo hsim_indC_spec. ss. econs 8; eauto. des. esplits; eauto. gbase. eauto. }
+    { guclo hsim_indC_spec. ss. econs 9; eauto. gbase. eauto. }
+    { guclo hsim_indC_spec. ss. econs 10; eauto. gbase. eauto. }
+    { guclo hsim_indC_spec. ss. econs 11; eauto. des. esplits; eauto. gbase. eauto. }
+    { guclo hsim_indC_spec. ss. econs 12; eauto. gbase. eauto. }
+    { guclo hsim_indC_spec. ss. econs 13; eauto. gbase. eauto. }
+    { guclo hsim_indC_spec. ss. econs 14; eauto. gbase. eauto. }
+    { guclo hsim_indC_spec. ss. econs 15; eauto. gbase. eauto. }
+    { gstep. econs 16; eauto. i. gbase. eauto. }
+  Qed.
+
+  Lemma hsimC_uclo r g:
+    @hsimC (gpaco9 (_hsim) (cpn9 _hsim) r g) (gupaco9 (_hsim) (cpn9 _hsim) g) <9= gpaco9 (_hsim) (cpn9 _hsim) r g.
+  Proof.
+    i. eapply hsimC_spec in PR.  ss.
+    eapply gpaco9_gpaco; [eauto with paco|].
+    eapply gpaco9_mon; eauto. i. eapply gupaco9_mon; eauto.
+  Qed.
+
   Variant hbindC (r: forall R_src R_tgt
                             (Q: Any.t -> Any.t -> R_src -> R_tgt -> iProp)
                             (ctx: Σ),
@@ -1038,8 +1122,6 @@ Section SIM.
   Proof. ii. inv IN; econs; et. Qed.
   Hint Resolve hbindC_mon: paco.
 
-  Lemma hsim_clo:
-
   Lemma hbindC_spec: hbindC <10= gupaco9 (_hsim) (cpn9 _hsim).
   Proof.
     eapply grespect_uclo.
@@ -1057,896 +1139,83 @@ Section SIM.
     { gstep. econs 2; eauto. i. hexploit POST; eauto. i.
       gbase. eapply rclo9_clo_base. left. econs; eauto.
     }
-    { admit "". }
+    { eapply hsimC_uclo. econs 3; eauto. }
     { des. gstep. econs 4; eauto. esplits; eauto. i.
       hexploit SIM; eauto. i. gbase. eapply rclo9_clo_base. left. econs; eauto.
     }
     { gstep. econs 5; eauto. i. gbase. eapply rclo9_clo_base. left. econs; eauto. }
-    { gstep. econs 6; eauto. }
-    { econs 7; eauto. }
-    { des. econs 8; eauto. }
-    { econs 9; eauto. i. hexploit SIM; eauto. i. des. eauto. }
-    { econs 10; eauto. i. hexploit SIM; eauto. i. des. eauto. }
-    { des. econs 11; eauto. }
-    { econs 12; eauto. }
-    { econs 13; eauto. }
-    { econs 14; eauto. }
-    { econs 15; eauto. }
-    { econs 16; eauto. eapply rclo9_clo_base. econs; eauto. }
+    { eapply hsimC_uclo. econs 6; eauto. }
+    { eapply hsimC_uclo. econs 7; eauto. }
+    { des. eapply hsimC_uclo. econs 8; eauto. }
+    { eapply hsimC_uclo. econs 9; eauto. i. hexploit SIM; eauto. i. des. esplits; eauto. }
+    { eapply hsimC_uclo. econs 10; eauto. i. hexploit SIM; eauto. i. des. esplits; eauto. }
+    { des. eapply hsimC_uclo. econs 11; eauto. }
+    { eapply hsimC_uclo. econs 12; eauto. }
+    { eapply hsimC_uclo. econs 13; eauto. }
+    { eapply hsimC_uclo. econs 14; eauto. }
+    { eapply hsimC_uclo. econs 15; eauto. }
+    { gstep. econs 16; eauto. gbase. eapply rclo9_clo_base. left. econs; eauto. }
   Qed.
 
-  Lemma hbindC_spec: hbindC <10= gupaco9 (_hsim) (cpn9 _hsim).
-  Proof.
-    eapply grespect9_uclo; eauto with paco.
-    econs; eauto with paco. i. inv PR. eapply GF in SIM.
-    cut (gpaco9 _hsim (cpn9 _hsim) bot9 (@_hsim (rclo9 (hbindC \10/ gupaco9 _hsim (cpn9 _hsim)) r))
-                x0 x1 x2 x3 x4 x5 x6 (st_src0, itr_src >>= ktr_src)
-                (st_tgt0, itr_tgt >>= ktr_tgt)).
-    { i. inv H. eapply rclo9_mon.
-      { eapply IN. }
-      { i. ss. des; ss. admit "". }
-    }
-    remember (st_src0, itr_src). remember (st_tgt0, itr_tgt).
-    revert st_src0 itr_src st_tgt0 itr_tgt Heqp Heqp0.
-    induction SIM using _hsim_ind2; i; clarify; ired_both.
-    { eapply rclo9_base. hexploit SIMK; eauto. i.
-      eapply GF in H. admit "ez".
-    }
-    { eapply rclo9_base. econs 2; eauto. i. hexploit POST; eauto. i.
-      eapply rclo9_clo_base. left. econs; eauto.
-    }
-    { admit "". }
-    { eapply rclo9_base. des. econs 4; eauto. esplits; eauto. i.
-      hexploit SIM; eauto. i. eapply rclo9_clo_base. left. econs; eauto.
-    }
-    { eapply rclo9_base. econs 5; eauto. i. eapply rclo9_clo_base. left. econs; eauto. }
-    { eapply rclo9_base. econs 6; eauto. }
-    { econs 7; eauto. }
-    { des. econs 8; eauto. }
-    { econs 9; eauto. i. hexploit SIM; eauto. i. des. eauto. }
-    { econs 10; eauto. i. hexploit SIM; eauto. i. des. eauto. }
-    { des. econs 11; eauto. }
-    { econs 12; eauto. }
-    { econs 13; eauto. }
-    { econs 14; eauto. }
-    { econs 15; eauto. }
-    { econs 16; eauto. eapply rclo9_clo_base. econs; eauto. }
-  Qed.
+  Variant hsplitC (r: forall R_src R_tgt
+                            (Q: Any.t -> Any.t -> R_src -> R_tgt -> iProp)
+                            (ctx: Σ),
+                     option Ord.t -> bool -> bool -> Any.t * itree hEs R_src -> Any.t * itree Es R_tgt -> Prop)
+          {R_src R_tgt}
+          (Q: Any.t -> Any.t -> R_src -> R_tgt -> iProp)
+          (ctx: Σ)
+    : option Ord.t -> bool -> bool -> Any.t * itree hEs R_src -> Any.t * itree Es R_tgt -> Prop :=
+  | hsplitC_intro
+      S_tgt
+      (P: Any.t -> Any.t -> S_tgt -> iProp)
+      fuel0 fuel1 f_src f_tgt st_src0 st_tgt0 itr_src itr_tgt ktr_tgt
+      (SIM: @r unit S_tgt (fun st_src st_tgt _ ret_tgt => P st_src st_tgt ret_tgt) ctx (Some fuel0) f_src f_tgt (st_src0, Ret tt) (st_tgt0, itr_tgt))
+      (SIMK: forall ctx1 st_src1 st_tgt1 ret_tgt
+                    (POST: current_iProp ctx1 (P st_src1 st_tgt1 ret_tgt)),
+          @r R_src R_tgt Q ctx1 (Some fuel1) false false (st_src1, itr_src) (st_tgt1, ktr_tgt ret_tgt))
+    :
+      hsplitC r Q ctx (Some (fuel1 + fuel0)%ord) f_src f_tgt (st_src0, itr_src) (st_tgt0, itr_tgt >>= ktr_tgt)
+  .
 
-  Lemma hbindC_spec: hbindC <10= gupaco9 (_hsim) (cpn9 _hsim).
+  Lemma hsplitC_mon:
+    monotone9 hsplitC.
+  Proof. ii. inv IN; econs; et. Qed.
+  Hint Resolve hsplitC_mon: paco.
+
+  Lemma hsplitC_spec: hsplitC <10= gupaco9 (_hsim) (cpn9 _hsim).
   Proof.
-    eapply wrespect9_uclo; eauto with paco.
+    eapply grespect_uclo.
     econs; eauto with paco. i. inv PR. eapply GF in SIM.
-    remember (st_src0, itr_src). remember (st_tgt0, itr_tgt).
-    revert st_src0 itr_src st_tgt0 itr_tgt Heqp Heqp0.
+    remember (st_src0, Ret tt). remember (st_tgt0, itr_tgt). remember (Some fuel0).
+    revert fuel0 st_src0 st_tgt0 itr_tgt Heqp Heqp0 Heqo0.
     induction SIM using _hsim_ind2; i; clarify; ired_both.
     { hexploit SIMK; eauto. i.
-      eapply GF in H. admit "ez".
+      eapply GF in H. guclo hflagC_spec. econs.
+      2:{ instantiate (1:=false). ss. }
+      2:{ instantiate (1:=false). ss. }
+      2:{ instantiate (1:=(Some fuel1)). ss. apply OrdArith.add_base_l. }
+      gstep. eapply _hsim_mon; eauto. i. gbase. eapply rclo9_base. auto.
     }
-    { econs 2; eauto. i. hexploit POST; eauto. i.
-      eapply rclo9_clo_base. econs; eauto.
+    { apply f_equal with (f:=_observe) in H0. ss. }
+    { apply f_equal with (f:=_observe) in H0. ss. }
+    { des. gstep. econs 4; eauto. esplits; eauto.
+      { eapply OrdArith.lt_add_r. eauto. }
+      i. hexploit SIM; eauto. i. gbase. eapply rclo9_clo_base. left. econs; eauto.
     }
-    { econs 3; eauto. }
-    { des. econs 4; eauto. esplits; eauto. i.
-      hexploit SIM; eauto. i. eapply rclo9_clo_base. econs; eauto.
-    }
-    { econs 5; eauto. i. i. eapply rclo9_clo_base. econs; eauto. }
-    { econs 6; eauto. }
-    { econs 7; eauto. }
-    { des. econs 8; eauto. }
-    { econs 9; eauto. i. hexploit SIM; eauto. i. des. eauto. }
-    { econs 10; eauto. i. hexploit SIM; eauto. i. des. eauto. }
-    { des. econs 11; eauto. }
-    { econs 12; eauto. }
-    { econs 13; eauto. }
-    { econs 14; eauto. }
-    { econs 15; eauto. }
-    { econs 16; eauto. eapply rclo9_clo_base. econs; eauto. }
+    { apply f_equal with (f:=_observe) in H0. ss. }
+    { eapply hsimC_uclo. econs 7; eauto. }
+    { apply f_equal with (f:=_observe) in H0. ss. }
+    { eapply hsimC_uclo. econs 9; eauto. i. hexploit SIM; eauto. i. des. esplits; eauto. }
+    { apply f_equal with (f:=_observe) in H0. ss. }
+    { des. eapply hsimC_uclo. econs 11; eauto. }
+    { apply f_equal with (f:=_observe) in H0. ss. }
+    { eapply hsimC_uclo. econs 13; eauto. }
+    { apply f_equal with (f:=_observe) in H0. ss. }
+    { eapply hsimC_uclo. econs 15; eauto. }
+    { gstep. econs 16; eauto. gbase. eapply rclo9_clo_base. left. econs; eauto. }
   Qed.
+
+(* TODO: frame, wand *)
+
 
 End SIM.
-
-
-Section HLEMMAS.
-  Context `{Σ: GRA.t}.
-  Local Opaque GRA.to_URA.
-
-  Variant mk_wf (A: Type)
-          (R: A -> Any.t -> Any.t -> iProp)
-    : A -> Any.t * Any.t -> Prop :=
-  | mk_wf_intro
-      a
-      mr_src mp_src mp_tgt
-      (RSRC: URA.wf mr_src -> R a mp_src mp_tgt mr_src)
-    :
-      mk_wf R a ((Any.pair mp_src mr_src↑), mp_tgt)
-  .
-
-  Definition inv_wf
-             `{@GRA.inG invRA Σ}
-             A
-             (R: A -> Any.t -> Any.t -> iProp)
-    : _ -> (Any.t * Any.t -> Prop) :=
-    @mk_wf
-      (A + Any.t * Any.t)%type
-      (fun a' mp_src mp_tgt =>
-         match a' with
-         | inl a => R a mp_src mp_tgt
-         | inr (mp_src1, mp_tgt1) => inv_closed ** ⌜mp_src1 = mp_src /\ mp_tgt1 = mp_tgt⌝
-         end)%I
-  .
-
-  Lemma hcall_clo_ord_weaken'
-        (fsp1: fspec)
-        (x: shelve__ fsp1.(meta))
-
-        A (a0: shelve__ A) FR
-
-        (le: A -> A -> Prop) mn r rg a n m mr_src0 mp_src0
-        (fsp0: fspec)
-        mp_tgt0 k_tgt k_src
-        fn tbr ord_cur varg_src varg_tgt
-        (R: A -> Any.t -> Any.t -> iProp)
-        (eqr: Any.t -> Any.t -> Any.t -> Any.t -> Prop)
-
-        (WEAKER: fspec_weaker fsp1 fsp0)
-
-        ctx0 I
-        (ACC: current_iProp ctx0 I)
-
-        (UPDATABLE:
-           I ⊢ #=> (FR ** R a0 mp_src0 mp_tgt0 ** (fsp1.(precond) (Some mn) x varg_src varg_tgt: iProp)))
-
-        (PURE: ord_lt (fsp1.(measure) x) ord_cur /\
-               (tbr = true -> is_pure (fsp1.(measure) x)) /\ (tbr = false -> (fsp1.(measure) x) = ord_top))
-
-        (POST: forall (vret_tgt : Any.t) (mr_src1: Σ) (mp_src1 mp_tgt1 : Any.t) a1
-                      (vret_src: Any.t)
-                      (WLE: le a0 a1)
-                      ctx1
-                      (ACC: current_iProp ctx1 (FR ** R a1 mp_src1 mp_tgt1 ** fsp1.(postcond) (Some mn) x vret_src vret_tgt))
-          ,
-                gpaco8 (_sim_itree (mk_wf R) le) (cpn8 (_sim_itree (mk_wf R) le)) rg rg _ _ eqr true true a
-                       (Any.pair mp_src1 mr_src1↑, k_src (ctx1, vret_src)) (mp_tgt1, k_tgt vret_tgt))
-    :
-      gpaco8 (_sim_itree (mk_wf R) le) (cpn8 (_sim_itree (mk_wf R) le)) r rg _ _ eqr m n a
-             (Any.pair mp_src0 mr_src0, (HoareCall mn tbr ord_cur fsp0 fn varg_src) ctx0 >>= k_src)
-             (mp_tgt0, trigger (Call fn varg_tgt) >>= k_tgt)
-  .
-  Proof.
-    subst. unfold HoareCall, mput, mget, assume, guarantee.
-    ired_both. apply sim_itreeC_spec. econs.
-    hexploit (WEAKER x). i. des.
-    assert (exists mr_src0' rarg_src fr_src0',
-               (<<UPDATABLE: URA.wf (ctx0 ⋅ (mr_src0' ⋅ (rarg_src ⋅ fr_src0')))>>) /\
-               (<<RSRC: R a0 mp_src0 mp_tgt0 mr_src0'>>) /\
-               (<<FRS: FR fr_src0'>>) /\
-               (<<PRE: fsp0.(precond) (Some mn) x_tgt varg_src varg_tgt rarg_src>>)).
-    { inv ACC. uipropall. hexploit UPDATABLE.
-      { eapply URA.wf_mon. eapply GWF. }
-      { eapply IPROP. }
-      { et. }
-      i. des. subst.
-      hexploit PRE; et. i. uipropall. hexploit (H0 b); et.
-      { eapply URA.wf_mon in H. rewrite URA.add_comm in H. eapply URA.wf_mon in H. auto. }
-      { instantiate (1:=a2 ⋅ b0 ⋅ ctx0).
-        replace (b ⋅ (a2 ⋅ b0 ⋅ ctx0)) with (a2 ⋅ b0 ⋅ b ⋅ ctx0); auto. r_solve. }
-      i. des. esplits; et.
-      { replace (ctx0 ⋅ (b0 ⋅ (r1 ⋅ a2))) with (r1 ⋅ (a2 ⋅ b0 ⋅ ctx0)); auto. r_solve. }
-    }
-    des. exists (rarg_src, fr_src0', mr_src0').
-    repeat (ired_both; apply sim_itreeC_spec; econs). unshelve esplits; eauto.
-    { r_wf UPDATABLE0. }
-    repeat (ired_both; apply sim_itreeC_spec; econs). exists x_tgt.
-    repeat (ired_both; apply sim_itreeC_spec; econs). exists varg_tgt.
-    repeat (ired_both; apply sim_itreeC_spec; econs). unshelve esplits; eauto.
-    repeat (ired_both; apply sim_itreeC_spec; econs). unshelve esplits; eauto.
-    { r in MEASURE. des_ifs; ss; des_ifs. eapply Ord.le_lt_lt; et. }
-    { i. spc PURE0. r in MEASURE. des_ifs; ss; des_ifs. }
-    { i. spc PURE1. r in MEASURE. des_ifs; ss; des_ifs. }
-    repeat (ired_both; apply sim_itreeC_spec; econs).
-    { econs; eauto. }
-    i. repeat (ired_both; apply sim_itreeC_spec; econs). i. destruct x0.
-    repeat (ired_both; apply sim_itreeC_spec; econs). inv WF.
-    repeat (ired_both; apply sim_itreeC_spec; econs). i.
-    repeat (ired_both; apply sim_itreeC_spec; econs). i.
-    repeat (ired_both; apply sim_itreeC_spec; econs). i.
-    ired_both. eapply POST; eauto. hexploit POST0. i.
-    uipropall. hexploit (H c); et.
-    { eapply URA.wf_mon. instantiate (1:=fr_src0' ⋅ c0 ⋅ mr_src). r_wf x0. }
-    { instantiate (1:=fr_src0' ⋅ c0 ⋅ mr_src). r_wf x0. }
-    i. des. econs.
-    { instantiate (1:=fr_src0' ⋅ mr_src ⋅ r1). r_wf H0. }
-    esplits; et.
-    eapply RSRC0.
-    eapply URA.wf_mon. instantiate (1:=r1 ⋅ fr_src0' ⋅ c0). r_wf H0.
-  Qed.
-
-  Lemma hcall_clo_ord_weaken
-        Hns Rn Invn
-        (fsp1: fspec)
-        (x: shelve__ fsp1.(meta))
-
-        A (a0: shelve__ A)
-
-        (le: A -> A -> Prop) mn r rg a n m mr_src0 mp_src0
-        (fsp0: fspec)
-        mp_tgt0 k_tgt k_src
-        fn tbr ord_cur varg_src varg_tgt
-        (R: A -> Any.t -> Any.t -> iProp)
-        (eqr: Any.t -> Any.t -> Any.t -> Any.t -> Prop)
-
-        (WEAKER: fspec_weaker fsp1 fsp0)
-
-        ctx0 l
-        (ACC: current_iPropL ctx0 l)
-
-        (UPDATABLE:
-           from_iPropL (fst (alist_pops Hns l)) ⊢ #=> (R a0 mp_src0 mp_tgt0 ** (fsp1.(precond) (Some mn) x varg_src varg_tgt: iProp)))
-
-        (PURE: ord_lt (fsp1.(measure) x) ord_cur /\
-               (tbr = true -> is_pure (fsp1.(measure) x)) /\ (tbr = false -> (fsp1.(measure) x) = ord_top))
-
-        (POST: forall (vret_tgt : Any.t) (mr_src1: Σ) (mp_src1 mp_tgt1 : Any.t) a1
-                      (vret_src: Any.t)
-                      (WLE: le a0 a1)
-                      ctx1
-                      (ACC: current_iPropL ctx1 ((Invn, R a1 mp_src1 mp_tgt1) :: (Rn, fsp1.(postcond) (Some mn) x vret_src vret_tgt) :: snd (alist_pops Hns l)))
-          ,
-            gpaco8 (_sim_itree (mk_wf R) le) (cpn8 (_sim_itree (mk_wf R) le)) rg rg _ _ eqr true true a
-                   (Any.pair mp_src1 mr_src1↑, k_src (ctx1, vret_src)) (mp_tgt1, k_tgt vret_tgt))
-    :
-      gpaco8 (_sim_itree (mk_wf R) le) (cpn8 (_sim_itree (mk_wf R) le)) r rg _ _ eqr m n a
-             (Any.pair mp_src0 mr_src0, (HoareCall mn tbr ord_cur fsp0 fn varg_src) ctx0 >>= k_src)
-             (mp_tgt0, trigger (Call fn varg_tgt) >>= k_tgt)
-  .
-  Proof.
-    subst. eapply hcall_clo_ord_weaken'; et.
-    { instantiate (2:=from_iPropL (snd (alist_pops Hns l))).
-      etrans.
-      { eapply iPropL_alist_pops. }
-      iIntros "[H0 H1]".
-      iPoseProof (UPDATABLE with "H0") as "> [H0 H2]".
-      iModIntro. iFrame.
-    }
-    i. eapply POST; et. red. ss.
-    eapply current_iProp_entail; et.
-    iIntros "[[H0 H1] H2]". iFrame.
-  Qed.
-
-  Lemma hcall_clo_weaken
-        Hns Rn Invn
-        (fsp1: fspec)
-        (x: shelve__ fsp1.(meta))
-
-        A (a0: shelve__ A)
-
-        (le: A -> A -> Prop) mn r rg a n m mr_src0 mp_src0
-        (fsp0: fspec)
-        mp_tgt0 k_tgt k_src
-        fn tbr ord_cur varg_src varg_tgt
-        (R: A -> Any.t -> Any.t -> iProp)
-        (eqr: Any.t -> Any.t -> Any.t -> Any.t -> Prop)
-
-        (WEAKER: fspec_weaker fsp1 fsp0)
-
-        ctx0 l
-        (ACC: current_iPropL ctx0 l)
-
-        (UPDATABLE:
-           from_iPropL (fst (alist_pops Hns l)) ⊢ #=> (R a0 mp_src0 mp_tgt0 ** (fsp1.(precond) (Some mn) x varg_src varg_tgt: iProp)))
-
-        (PURE: ord_lt (fsp1.(measure) x) ord_cur /\
-               (tbr = true -> is_pure (fsp1.(measure) x)) /\ (tbr = false -> (fsp1.(measure) x) = ord_top))
-
-        (POST: forall (vret_tgt : Any.t) (mr_src1: Σ) (mp_src1 mp_tgt1 : Any.t) a1
-                      (vret_src: Any.t)
-                      (WLE: le a0 a1)
-                      ctx1
-                      (ACC: current_iPropL ctx1 (@cons (prod string (bi_car iProp)) (Invn, R a1 mp_src1 mp_tgt1) (@cons (prod string (bi_car iProp)) (Rn, fsp1.(postcond) (Some mn) x vret_src vret_tgt) (snd (alist_pops Hns l)))))
-          ,
-            gpaco8 (_sim_itree (mk_wf R) le) (cpn8 (_sim_itree (mk_wf R) le)) rg rg _ _ eqr true true a
-                   (Any.pair mp_src1 mr_src1↑, k_src (ctx1, vret_src)) (mp_tgt1, k_tgt vret_tgt))
-    :
-      gpaco8 (_sim_itree (mk_wf R) le) (cpn8 (_sim_itree (mk_wf R) le)) r rg _ _ eqr m n a
-             (Any.pair mp_src0 mr_src0, (HoareCall mn tbr ord_cur fsp0 fn varg_src) ctx0 >>= k_src)
-             (mp_tgt0, trigger (Call fn varg_tgt) >>= k_tgt)
-  .
-  Proof.
-    eapply (@hcall_clo_ord_weaken _ _ _); eauto.
-  Qed.
-
-  Lemma hcall_clo
-        Hns Rn Invn
-        X (x: shelve__ X)
-        A (a0: shelve__ A)
-
-        (D: X -> ord)
-        (P: option mname -> X -> Any.t -> Any.t -> Σ -> Prop)
-        (Q: option mname -> X -> Any.t -> Any.t -> Σ -> Prop)
-        (le: A -> A -> Prop) mn r rg a n m mr_src0 mp_src0
-        mp_tgt0 k_tgt k_src
-        fn tbr ord_cur varg_src varg_tgt
-        (R: A -> Any.t -> Any.t -> iProp)
-        (eqr: Any.t -> Any.t -> Any.t -> Any.t -> Prop)
-
-        ctx0 l
-        (ACC: current_iPropL ctx0 l)
-
-        (UPDATABLE:
-           from_iPropL (fst (alist_pops Hns l)) ⊢ #=> (R a0 mp_src0 mp_tgt0 ** (P (Some mn) x varg_src varg_tgt: iProp)))
-
-        (PURE: ord_lt (D x) ord_cur /\
-               (tbr = true -> is_pure (D x)) /\ (tbr = false -> (D x) = ord_top))
-
-        (POST: forall (vret_tgt : Any.t) (mr_src1: Σ) (mp_src1 mp_tgt1 : Any.t) a1
-                      (vret_src: Any.t)
-                      (WLE: le a0 a1)
-                      ctx1
-                      (ACC: current_iPropL ctx1 (@cons (prod string (bi_car iProp)) (Invn, R a1 mp_src1 mp_tgt1) (@cons (prod string (bi_car iProp)) (Rn, Q (Some mn) x vret_src vret_tgt) (snd (alist_pops Hns l)))))
-          ,
-                gpaco8 (_sim_itree (mk_wf R) le) (cpn8 (_sim_itree (mk_wf R) le)) rg rg _ _ eqr true true a
-                       (Any.pair mp_src1 mr_src1↑, k_src (ctx1, vret_src)) (mp_tgt1, k_tgt vret_tgt))
-    :
-      gpaco8 (_sim_itree (mk_wf R) le) (cpn8 (_sim_itree (mk_wf R) le)) r rg _ _ eqr m n a
-             (Any.pair mp_src0 mr_src0, (HoareCall mn tbr ord_cur (mk_fspec D P Q) fn varg_src) ctx0 >>= k_src)
-             (mp_tgt0, trigger (Call fn varg_tgt) >>= k_tgt)
-  .
-  Proof.
-    eapply hcall_clo_weaken; eauto.
-    { refl. }
-    { eauto. }
-    { eauto. }
-    { eauto. }
-  Qed.
-
-  Lemma harg_clo
-        A Rn Invn
-        mn r rg
-        X (P: option mname -> X -> Any.t -> Any.t -> Σ -> Prop) varg
-        mpr_src mp_tgt f_tgt k_src
-        a (le: A -> A -> Prop)
-        (R: A -> Any.t -> Any.t -> iProp)
-        (eqr: Any.t -> Any.t -> Any.t -> Any.t -> Prop)
-        (WF: mk_wf R a (mpr_src, mp_tgt))
-        m n
-        (ARG:
-           forall x varg_src
-                  ctx (mr_src: Σ) mp_src
-                  (ACC: current_iPropL ctx (@cons (prod string (bi_car iProp)) (Rn, P mn x varg_src varg) (@cons (prod string (bi_car iProp)) (Invn, R a mp_src mp_tgt) (@nil (prod string (bi_car iProp)))))),
-             gpaco8 (_sim_itree (mk_wf R) le) (cpn8 (_sim_itree (mk_wf R) le)) r rg _ _ eqr true n a
-                    (Any.pair mp_src mr_src↑, k_src (ctx, ((mn, x), varg_src)))
-                    (mp_tgt, f_tgt))
-    :
-      gpaco8 (_sim_itree (mk_wf R) le) (cpn8 (_sim_itree (mk_wf R) le)) r rg _ _ eqr m n a
-             (mpr_src, (HoareFunArg P (mn, varg) >>= k_src))
-             (mp_tgt, f_tgt)
-  .
-  Proof.
-    inv WF.
-    unfold HoareFunArg, mput, mget, assume, guarantee.
-    repeat (ired_both; apply sim_itreeC_spec; econs). intro x.
-    repeat (ired_both; apply sim_itreeC_spec; econs). intro varg_src.
-    repeat (ired_both; apply sim_itreeC_spec; econs). intros (rarg_src, ctx).
-    repeat (ired_both; apply sim_itreeC_spec; econs). intros VALID.
-    repeat (ired_both; apply sim_itreeC_spec; econs). intro PRE.
-    ired_both. eapply ARG; et.
-    red. econs.
-    { instantiate (1:=rarg_src ⋅ mr_src). r_wf VALID. }
-    { ss. red. uipropall. esplits; et.
-      { rewrite URA.unit_id. et. }
-      { eapply RSRC; et. eapply URA.wf_mon. instantiate (1:=(ctx ⋅ rarg_src)). r_wf VALID. }
-      { red. uipropall. }
-    }
-  Qed.
-
-  Lemma hret_clo
-        A (a: shelve__ A)
-        mn r rg n m mr_src mp_src a0
-        X (Q: option mname -> X -> Any.t -> Any.t -> Σ -> Prop)
-        x vret_src vret_tgt
-        mp_tgt
-        (le: A -> A -> Prop)
-        (eqr: Any.t -> Any.t -> Any.t -> Any.t -> Prop)
-        (R: A -> Any.t -> Any.t -> iProp)
-
-        ctx l
-        (ACC: current_iPropL ctx l)
-
-        (WLE: le a0 a)
-
-        (UPDATABLE:
-           (from_iPropL l) ⊢ #=> (R a mp_src mp_tgt ** (Q mn x vret_src vret_tgt: iProp)))
-
-        (EQ: forall (mr_src1: Σ) (WLE: le a0 a) (WF: mk_wf R a (Any.pair mp_src mr_src1↑, mp_tgt)),
-            eqr (Any.pair mp_src mr_src1↑) mp_tgt vret_tgt vret_tgt)
-    :
-      gpaco8 (_sim_itree (mk_wf R) le) (cpn8 (_sim_itree (mk_wf R) le)) r rg _ _ eqr m n a0
-             (Any.pair mp_src mr_src, (HoareFunRet Q mn x (ctx, vret_src)))
-             (mp_tgt, (Ret vret_tgt))
-  .
-  Proof.
-    subst. unfold HoareFunRet, mput, mget, guarantee.
-    repeat (ired_both; apply sim_itreeC_spec; econs). exists vret_tgt.
-    repeat (ired_both; apply sim_itreeC_spec; econs).
-    assert (exists mr_src1 rret_src,
-               (<<UPDATABLE: URA.wf (ctx ⋅ (mr_src1 ⋅ rret_src))>>) /\
-               (<<RSRC: R a mp_src mp_tgt mr_src1>>) /\
-               (<<PRE: Q mn x vret_src vret_tgt rret_src>>)).
-    { red in ACC. inv ACC. uipropall.
-      hexploit (UPDATABLE r0); et.
-      { eapply URA.wf_mon; et. }
-      i. des. subst. exists a1, b. splits; et.
-      replace (ctx ⋅ (a1 ⋅ b)) with (a1 ⋅ b ⋅ ctx); et.
-      r_solve.
-    }
-    des. exists (rret_src, mr_src1).
-    repeat (ired_both; apply sim_itreeC_spec; econs).
-    repeat (ired_both; apply sim_itreeC_spec; econs). unshelve esplits.
-    { r_wf UPDATABLE0. }
-    repeat (ired_both; apply sim_itreeC_spec; econs). unshelve esplits; eauto.
-    repeat (ired_both; apply sim_itreeC_spec; econs).
-    eapply EQ; et. econs; et.
-  Qed.
-
-  Lemma APC_start_clo
-        (at_most: Ord.t)
-        (o: ord)
-        A mn r rg a m n mp_src0
-        k_src
-        (wf: A -> Any.t * Any.t -> Prop)
-        (le: A -> A -> Prop)
-        (eqr: Any.t -> Any.t -> Any.t -> Any.t -> Prop)
-        stb itr_tgt ctx
-
-        (POST: gpaco8 (_sim_itree wf le) (cpn8 (_sim_itree wf le)) r rg _ _ eqr true n a
-                      (mp_src0,
-                       (interp_hCallE_tgt mn stb o (_APC at_most) ctx)>>= k_src)
-                      (itr_tgt))
-    :
-      gpaco8 (_sim_itree wf le) (cpn8 (_sim_itree wf le)) r rg _ _ eqr m n a
-             (mp_src0,
-              (interp_hCallE_tgt mn stb o APC ctx) >>= k_src)
-             (itr_tgt).
-  Proof.
-    subst. unfold APC. destruct itr_tgt.
-    ired_both. apply sim_itreeC_spec. eapply sim_itreeC_choose_src.
-    exists at_most.
-    repeat (ired_both; apply sim_itreeC_spec; econs).
-    ired_both. et.
-    Unshelve. all: ss.
-  Qed.
-
-  Lemma APC_stop_clo
-        (o: ord)
-        A mn r rg a n m mp_src0
-        k_src
-        (at_most: Ord.t)
-        (wf: A -> Any.t * Any.t -> Prop)
-        (le: A -> A -> Prop)
-        (eqr: Any.t -> Any.t -> Any.t -> Any.t -> Prop)
-        stb itr_tgt ctx
-
-        (POST: gpaco8 (_sim_itree wf le) (cpn8 (_sim_itree wf le)) r rg _ _ eqr true n a
-                      (mp_src0, k_src (ctx, ()))
-                      (itr_tgt))
-    :
-      gpaco8 (_sim_itree wf le) (cpn8 (_sim_itree wf le)) r rg _ _ eqr m n a
-              (mp_src0,
-              (interp_hCallE_tgt mn stb o (_APC at_most) ctx) >>= k_src)
-             (itr_tgt).
-  Proof.
-    subst. destruct itr_tgt.
-    rewrite unfold_APC. ired_l. apply sim_itreeC_spec. eapply sim_itreeC_choose_src.
-    exists true. ired_l. apply sim_itreeC_spec. eapply sim_itreeC_tau_src.
-    ired_both. et.
-  Qed.
-
-  Lemma APC_step_clo
-        (fn: gname) (args: Any.t) (next: Ord.t)
-
-        (o: ord)
-        A mn r rg a n m mp_src0
-        k_src ctx0
-        (at_most: Ord.t)
-        (wf: A -> Any.t * Any.t -> Prop)
-        (le: A -> A -> Prop)
-        (eqr: Any.t -> Any.t -> Any.t -> Any.t -> Prop)
-        stb itr_tgt
-
-        (fsp: fspec)
-        (FIND: stb fn = Some fsp)
-        (NEXT: (next < at_most)%ord)
-
-        (POST: gpaco8 (_sim_itree wf le) (cpn8 (_sim_itree wf le)) r rg _ _ eqr true n a
-                      (mp_src0,
-                       ('(ctx1, _) <- (HoareCall mn true o fsp fn args ctx0);;
-                        Tau (ITree.bind (interp_hCallE_tgt mn stb o (_APC next) ctx1) k_src)))
-                      (itr_tgt))
-    :
-      gpaco8 (_sim_itree wf le) (cpn8 (_sim_itree wf le)) r rg _ _ eqr m n a
-             (mp_src0, (interp_hCallE_tgt mn stb o (_APC at_most) ctx0) >>= k_src)
-             (itr_tgt).
-  Proof.
-    subst. destruct itr_tgt.
-    rewrite unfold_APC. ired_l. apply sim_itreeC_spec. eapply sim_itreeC_choose_src.
-    exists false. ired_l. apply sim_itreeC_spec. eapply sim_itreeC_tau_src.
-    ired_l. apply sim_itreeC_spec. eapply sim_itreeC_choose_src.
-    exists next. ired_l. apply sim_itreeC_spec. eapply sim_itreeC_tau_src.
-    ired_l. unfold guarantee. ired_l. apply sim_itreeC_spec. eapply sim_itreeC_choose_src.
-    split.
-    { auto. }
-    ired_l. apply sim_itreeC_spec. eapply sim_itreeC_tau_src.
-    ired_l. apply sim_itreeC_spec. eapply sim_itreeC_choose_src.
-    exists (fn, args).
-    ired_l. apply sim_itreeC_spec. eapply sim_itreeC_tau_src.
-    ired_l. ss. rewrite FIND. ss. subst. ired_l.
-    ss. ired_l.
-    match goal with
-    | [SIM: gpaco8 _ _ _ _ _ _ _ _ _ _ ?i0 _ |- gpaco8 _ _ _ _ _ _ _ _ _ _ ?i1 _] =>
-      replace i1 with i0; et
-    end.
-    f_equal. grind.
-  Qed.
-
-  Lemma trivial_init_clo
-        A wf (le: A -> A -> Prop) r rg w arg mrp_src mp_tgt itr_tgt mn stb body RR
-        m n
-        (INIT:
-           gpaco8 (_sim_itree wf le) (cpn8 (_sim_itree wf le)) r rg Any.t Any.t
-                  RR true n w
-                  (mrp_src, fun_to_tgt mn stb (mk_specbody fspec_trivial body) arg)
-                  (mp_tgt, itr_tgt))
-    :
-      gpaco8 (_sim_itree wf le) (cpn8 (_sim_itree wf le)) r rg Any.t Any.t
-             RR m n w
-             (mrp_src, KModSem.disclose_ksb_tgt mn stb (ksb_trivial body) arg)
-             (mp_tgt, itr_tgt).
-  Proof.
-    unfold KModSem.disclose_ksb_tgt.
-    apply sim_itreeC_spec. econs; eauto. i. destruct x; et.
-  Qed.
-
-End HLEMMAS.
-
-
-Ltac prep := ired_both.
-
-Ltac _force_l :=
-  prep;
-  match goal with
-  | [ |- (gpaco8 (_sim_itree _ _) _ _ _ _ _ _ _ _ _ (_, unwrapN ?ox >>= _) (_, _)) ] =>
-    let tvar := fresh "tmp" in
-    let thyp := fresh "TMP" in
-    remember (unwrapN ox) as tvar eqn:thyp; unfold unwrapN in thyp; subst tvar;
-    let name := fresh "_UNWRAPN" in
-    destruct (ox) eqn:name; [|exfalso]; cycle 1
-  | [ |- (gpaco8 (_sim_itree _ _) _ _ _ _ _ _ _ _ _ (_, guarantee ?P >>= _) (_, _)) ] =>
-    let tvar := fresh "tmp" in
-    let thyp := fresh "TMP" in
-    remember (guarantee P) as tvar eqn:thyp; unfold guarantee in thyp; subst tvar;
-    let name := fresh "_GUARANTEE" in
-    destruct (classic P) as [name|name]; [ired_both; apply sim_itreeC_spec; eapply sim_itreeC_choose_src; [exists name]|contradict name]; cycle 1
-
-  | [ |- (gpaco8 (_sim_itree _ _) _ _ _ _ _ _ _ _ _ (_, ITree.bind' _ (interp _ guarantee ?P) (_, _))) ] =>
-    let tvar := fresh "tmp" in
-    let thyp := fresh "TMP" in
-    remember (guarantee P) as tvar eqn:thyp; unfold guarantee in thyp; subst tvar;
-    let name := fresh "_GUARANTEE" in
-    destruct (classic P) as [name|name]; [ired_both; apply sim_itreeC_spec; eapply sim_itreeC_choose_src; [exists name]|contradict name]; cycle 1
-
-   (* TODO: handle interp_hCallE_tgt better and remove this case *)
-  | [ |- (gpaco8 (_sim_itree _ _) _ _ _ _ _ _ _ _ _ (_, ITree.bind' _ (interp _ (guarantee ?P ))) (_, _)) ] =>
-    let tvar := fresh "tmp" in
-    let thyp := fresh "TMP" in
-    remember (guarantee P) as tvar eqn:thyp; unfold guarantee in thyp; subst tvar;
-    let name := fresh "_GUARANTEE" in
-    destruct (classic P) as [name|name]; [ired_both; apply sim_itreeC_spec; eapply sim_itreeC_choose_src; [exists name]|contradict name]; cycle 1; clear name
-
-  | [ |- (gpaco8 (_sim_itree _ _) _ _ _ _ _ _ _ _ _ (_, ?i_src) (_, ?i_tgt)) ] =>
-    seal i_tgt; apply sim_itreeC_spec; econs; unseal i_tgt
-  end
-.
-
-Ltac _force_r :=
-  prep;
-  match goal with
-  | [ |- (gpaco8 (_sim_itree _ _) _ _ _ _ _ _ _ _ _ (_, _) (_, unwrapU ?ox >>= _)) ] =>
-    let tvar := fresh "tmp" in
-    let thyp := fresh "TMP" in
-    remember (unwrapU ox) as tvar eqn:thyp; unfold unwrapU in thyp; subst tvar;
-    let name := fresh "_UNWRAPU" in
-    destruct (ox) eqn:name; [|exfalso]; cycle 1
-  | [ |- (gpaco8 (_sim_itree _ _) _ _ _ _ _ _ _ _ _ (_, _) (_, assume ?P >>= _)) ] =>
-    let tvar := fresh "tmp" in
-    let thyp := fresh "TMP" in
-    remember (assume P) as tvar eqn:thyp; unfold assume in thyp; subst tvar;
-    let name := fresh "_ASSUME" in
-    destruct (classic P) as [name|name]; [ired_both; apply sim_itreeC_spec; eapply sim_itreeC_take_tgt; [exists name]|contradict name]; cycle 1
-
-  | [ |- (gpaco8 (_sim_itree _ _) _ _ _ _ _ _ _ _ _ (_, ?i_src) (_, ?i_tgt)) ] =>
-    seal i_src; apply sim_itreeC_spec; econs; unseal i_src
-  end
-.
-
-Ltac _step :=
-  match goal with
-  (*** blacklisting ***)
-  (* | [ |- (gpaco5 (_sim_itree wf) _ _ _ _ (_, trigger (Choose _) >>= _) (_, ?i_tgt)) ] => idtac *)
-  | [ |- (gpaco8 (_sim_itree _ _) _ _ _ _ _ _ _ _ _ (_, triggerUB >>= _) (_, _)) ] =>
-    unfold triggerUB; ired_l; _step; done
-  | [ |- (gpaco8 (_sim_itree _ _) _ _ _ _ _ _ _ _ _ (_, unwrapU ?ox >>= _) (_, _)) ] =>
-    let tvar := fresh "tmp" in
-    let thyp := fresh "TMP" in
-    remember (unwrapU ox) as tvar eqn:thyp; unfold unwrapU in thyp; subst tvar;
-    let name := fresh "_UNWRAPU" in
-    destruct (ox) eqn:name; [|unfold triggerUB; ired_both; _force_l; ss; fail]
-  | [ |- (gpaco8 (_sim_itree _ _) _ _ _ _ _ _ _ _ _ (_, assume ?P >>= _) (_, _)) ] =>
-    let tvar := fresh "tmp" in
-    let thyp := fresh "TMP" in
-    remember (assume P) as tvar eqn:thyp; unfold assume in thyp; subst tvar;
-    let name := fresh "_ASSUME" in
-    ired_both; apply sim_itreeC_spec; eapply sim_itreeC_take_src; intro name
-
-  (*** blacklisting ***)
-  (* | [ |- (gpaco5 (_sim_itree wf) _ _ _ _ (_, _) (_, trigger (Take _) >>= _)) ] => idtac *)
-  | [ |- (gpaco8 (_sim_itree _ _) _ _ _ _ _ _ _ _ _ (_, triggerNB >>= _) (_, _)) ] =>
-    unfold triggerNB; ired_r; _step; done
-  | [ |- (gpaco8 (_sim_itree _ _) _ _ _ _ _ _ _ _ _ (_, _) (_, unwrapN ?ox >>= _)) ] =>
-    let tvar := fresh "tmp" in
-    let thyp := fresh "TMP" in
-    remember (unwrapN ox) as tvar eqn:thyp; unfold unwrapN in thyp; subst tvar;
-    let name := fresh "_UNWRAPN" in
-    destruct (ox) eqn:name; [|unfold triggerNB; ired_both; _force_r; ss; fail]
-  | [ |- (gpaco8 (_sim_itree _ _) _ _ _ _ _ _ _ _ _ (_, _) (_, guarantee ?P >>= _)) ] =>
-    let tvar := fresh "tmp" in
-    let thyp := fresh "TMP" in
-    remember (guarantee P) as tvar eqn:thyp; unfold guarantee in thyp; subst tvar;
-    let name := fresh "_GUARANTEE" in
-    ired_both; apply sim_itreeC_spec; eapply sim_itreeC_choose_tgt; intro name
-
-
-
-  | _ => (*** default ***)
-    eapply safe_sim_sim; econs; i
-  end;
-  match goal with
-  | [ |- exists (_: unit), _ ] => esplits; [eauto|..]; i
-  | [ |- exists _, _ ] => fail 1
-  | _ => idtac
-  end
-.
-Ltac _steps := repeat ((*** pre processing ***) prep; try _step; (*** post processing ***) simpl).
-
-Ltac steps := repeat ((*** pre processing ***) prep; try _step; (*** post processing ***) simpl; des_ifs_safe).
-Ltac force_l := _force_l.
-Ltac force_r := _force_r.
-
-Notation "wf n '------------------------------------------------------------------' src0 tgt0 '------------------------------------------------------------------' src1 '------------------------------------------------------------------' src2 tgt2"
-  :=
-    (gpaco8 (_sim_itree wf _) _ _ _ _ _ _ _ _ n ((Any.pair src0 src1), src2) (tgt0, tgt2))
-      (at level 60,
-       format "wf  n '//' '------------------------------------------------------------------' '//' src0 '//' tgt0 '//' '------------------------------------------------------------------' '//' src1 '//' '------------------------------------------------------------------' '//' src2 '//' '//' '//' tgt2 '//' ").
-
-Notation "wf n '------------------------------------------------------------------' src0 tgt0 '------------------------------------------------------------------' '------------------------------------------------------------------' src2 tgt2"
-  :=
-    (gpaco8 (_sim_itree wf _) _ _ _ _ _ _ _ _ n (src0, src2) (tgt0, tgt2))
-      (at level 60,
-       format "wf  n '//' '------------------------------------------------------------------' '//' src0 '//' tgt0 '//' '------------------------------------------------------------------' '//' '//' '------------------------------------------------------------------' '//' src2 '//' '//' '//' tgt2 '//' ").
-
-Section TEST.
-  Context `{Σ: GRA.t}.
-  Let wf := (mk_wf (fun (_ : unit) (_ _ : Any.t) => bi_pure True)).
-  Let le := fun (_ _: unit) => True.
-  Variable (srcs0 tgts0: Any.t).
-
-  Goal gpaco8 (_sim_itree wf le) (cpn8 (_sim_itree wf le)) bot8 bot8 Any.t Any.t (fun _ _ => eq) false false tt
-       (srcs0, triggerUB >>= idK) (tgts0, triggerUB >>= idK).
-  Proof.
-    steps.
-  Qed.
-
-  Goal gpaco8 (_sim_itree wf le) (cpn8 (_sim_itree wf le)) bot8 bot8 Any.t Any.t (fun _ _ => eq) false false tt
-       (srcs0, triggerNB >>= idK) (tgts0, triggerNB >>= idK).
-  Proof.
-    steps.
-  Qed.
-
-End TEST.
-
-
-Ltac astep_full _fn _args _next _n1 :=
-  eapply (@APC_step_clo _ _fn _args _next _n1);
-  [(try by ((try stb_tac); refl))|
-   oauto|
-  ].
-
-Ltac astep _fn _args :=
-  eapply (@APC_step_clo _ _fn _args);
-  [(try by ((try stb_tac); refl))|
-   oauto|
-  ].
-
-Ltac acatch :=
-  match goal with
-  | [ |- (gpaco8 (_sim_itree _ _) _ _ _ _ _ _ _ _ _ (_, _) (_, trigger (Call ?fn ?args) >>= _)) ] =>
-    astep fn args
-  end.
-
-Ltac astart _at_most :=
-  eapply (@APC_start_clo _ _at_most)
-.
-
-Ltac astop :=
-  match goal with
-  | [ |- (gpaco8 (_sim_itree _ _) _ _ _ _ _ _ _ _ _ (_, interp_hCallE_tgt _ _ _ APC _ >>= _) (_, _)) ] => astart 0
-  | _ => idtac
-  end;
-  eapply APC_stop_clo.
-
-Ltac init :=
-  let varg_src := fresh "varg_src" in
-  let mn := fresh "mn" in
-  let varg := fresh "varg" in
-  let EQ := fresh "EQ" in
-  let w := fresh "w" in
-  let mrp_src := fresh "mrp_src" in
-  let mp_tgt := fresh "mp_tgt" in
-  let WF := fresh "WF" in
-  split; ss; intros varg_src [mn varg] EQ w mrp_src mp_tgt WF;
-  try subst varg_src; cbn; ginit;
-  match goal with
-  | |- gpaco8 _ _ _ _ _ _ _ _ _ _ (_, KModSem.disclose_ksb_tgt _ _ (ksb_trivial _) _) _ =>
-    eapply trivial_init_clo;
-    try (unfold fun_to_tgt, cfunN, cfunU, KModSem.disclose_ksb_tgt, fun_to_tgt);
-    rewrite HoareFun_parse; simpl
-  | |- gpaco8 _ _ _ _ _ _ _ _ _ _ (_, KModSem.disclose_ksb_tgt _ _ _ _) _ =>
-    try (unfold fun_to_tgt, cfunN, cfunU, KModSem.disclose_ksb_tgt, fun_to_tgt);
-    simpl;
-    apply sim_itreeC_spec; apply sim_itreeC_take_src; intros [];rewrite HoareFun_parse; simpl
-  | |- _ =>
-    try (unfold fun_to_tgt, cfunN, cfunU; rewrite HoareFun_parse); simpl
-  end.
-
-Ltac harg :=
-  let PRE := constr:("PRE") in
-  let INV := constr:("INV") in
-  eapply (@harg_clo _ _ PRE INV);
-  [eassumption
-  |
-  ]; i.
-
-Tactic Notation "hret" uconstr(a) :=
-  eapply (@hret_clo _ _ a); unshelve_goal;
-  [eassumption
-  |
-  |start_ipm_proof
-  |try by (i; (try unfold lift_rel); esplits; et)
-  ].
-
-Tactic Notation "hcall" uconstr(x) uconstr(a) "with" constr(Hns) :=
-  let POST := get_fresh_name_tac "POST" in
-  let INV := get_fresh_name_tac "INV" in
-  let Hns := select_ihyps Hns in
-  eapply (@hcall_clo _ Hns POST INV _ x _ a);
-  unshelve_goal;
-  [eassumption
-  |start_ipm_proof
-  |
-  |on_current ltac:(fun H => try clear H); i; on_current ltac:(fun H => simpl in H)
-  ].
-
-Tactic Notation "hcall_weaken" uconstr(fsp) uconstr(x) uconstr(a) "with" constr(Hns) :=
-  let POST := get_fresh_name_tac "POST" in
-  let INV := get_fresh_name_tac "INV" in
-  let Hns := select_ihyps Hns in
-  eapply (@hcall_clo_weaken _ Hns POST INV fsp x _ a);
-  unshelve_goal;
-  [
-  |eassumption
-  |start_ipm_proof
-  |
-  |on_current ltac:(fun H => try clear H); i; on_current ltac:(fun H => simpl in H)
-  ].
-
-Ltac iarg :=
-  let PRE := constr:("PRE") in
-  let INV := constr:("INV") in
-  let CLOSED := constr:("☃CLOSED") in
-  eapply (@harg_clo _ _ PRE INV);
-  [eassumption
-  |
-  ];
-  i;
-  mDesSep PRE as CLOSED PRE;
-  match goal with
-  | [ |- (gpaco8 _ _ _ _ _ _ _ _ _ ?w _ _)] =>
-    destruct w as [?|[?mp_src ?mp_tgt]]; simpl;
-    [
-        |mAssertPure False; ss; iDestruct "INV" as "[INV _]"; iApply (inv_closed_unique with "☃CLOSED INV")
-    ]
-  end.
-
-Tactic Notation "icall_open" uconstr(x) "with" constr(Hns) :=
-  let POST := get_fresh_name_tac "POST" in
-  let INV := constr:("☃CLOSED") in
-  let Hns := select_ihyps Hns in
-  let Hns := constr:("☃CLOSED"::Hns) in
-  eapply (@hcall_clo _ Hns POST INV _ x _ (inr (_, _)));
-  unshelve_goal;
-  [eassumption
-  |start_ipm_proof; iSplitL "☃CLOSED"; [iModIntro; iSplitL "☃CLOSED"; [iExact "☃CLOSED"|ss]|]
-  |
-  |
-  on_current ltac:(fun H => try clear H);
-  intros ? ? ? ? [|[?mp_src ?mp_tgt]]; i; simpl;
-  on_current ltac:(fun H => simpl in H);
-  [exfalso; match goal with | H: inv_le _ _ _ |- _ => cbn in H; inv H end
-  |mDesSep "☃CLOSED" as "☃CLOSED" "☃TMP"; mPure "☃TMP" as [[] []]
-  ]
-  ].
-
-Tactic Notation "icall_weaken" uconstr(ftsp) uconstr(x) uconstr(a) "with" constr(Hns) :=
-  let POST := get_fresh_name_tac "POST" in
-  let INV := get_fresh_name_tac "INV" in
-  let CLOSED := constr:("☃CLOSED") in
-  let TMP := constr:("☃TMP") in
-  let Hns := select_ihyps Hns in
-  let Hns := constr:("☃CLOSED"::Hns) in
-  eapply (@hcall_clo_weaken _ Hns POST INV ftsp x _ (inl a));
-  unshelve_goal;
-  [|eassumption
-   |start_ipm_proof; iFrame "☃CLOSED"
-   |
-   |on_current ltac:(fun H => try clear H);
-    intros ? ? ? ? [|[?mp_src ?mp_tgt]]; i; simpl;
-    on_current ltac:(fun H => simpl in H);
-    [
-      mDesSep POST as "☃CLOSED" POST
-    |
-    mDesSep INV as "☃CLOSED" INV;
-    mDesSep POST as "☃TMP" POST;
-    mAssertPure False; [iApply (inv_closed_unique with "☃TMP ☃CLOSED")|ss]
-    ]
-  ].
-
-Tactic Notation "iret" uconstr(a) :=
-  eapply (@hret_clo _ _ (inl a)); unshelve_goal;
-  [eassumption
-  |
-  |start_ipm_proof; iFrame "☃CLOSED"
-  |try by (i; (try unfold lift_rel); esplits; et)
-  ].
-
-
-Global Opaque _APC APC interp interp_hCallE_tgt.
-
-Global Opaque HoareFun HoareFunArg HoareFunRet HoareCall.
-
-Definition __hide_mark A (a : A) : A := a.
-Lemma intro_hide_mark: forall A (a: A), a = __hide_mark a. refl. Qed.
-
-Ltac hide_k :=
-  match goal with
-  | [ |- (gpaco8 _ _ _ _ _ _ _ _ _ _ (_, ?isrc >>= ?ksrc) (_, ?itgt >>= ?ktgt)) ] =>
-    erewrite intro_hide_mark with (a:=ksrc);
-    erewrite intro_hide_mark with (a:=ktgt);
-    let name0 := fresh "__KSRC__" in set (__hide_mark ksrc) as name0; move name0 at top;
-    let name0 := fresh "__KTGT__" in set (__hide_mark ktgt) as name0; move name0 at top
-  end.
-
-Ltac unhide_k :=
-  do 2 match goal with
-  | [ H := __hide_mark _ |- _ ] => subst H
-  end;
-  rewrite <- ! intro_hide_mark
-.
-
-Ltac deflag :=
-  match goal with
-  | [ |- (gpaco8 _ _ _ _ _ _ _ true true _ _ _) ] =>
-    eapply sim_itree_progress_flag
-  | [ |- (gpaco8 _ _ _ _ _ _ _ _ _ _ _ _) ] =>
-    eapply sim_itree_flag_down
-  | _ => fail
-  end.
